standard reduction

Lambda.v
@@ -1,3 +1,6 @@
+Require Export Arith.
+Require Export Omega.
+
 Definition id : Type := nat.
 
 Inductive expr : Type :=
@@ -14,6 +17,8 @@ Inductive context : Type :=
   | app_l : context -> expr -> context
   | app_r : expr -> context -> context.
 
+Reserved Notation "E '[' e ']'" (at level 20).
+
 Fixpoint plug (ectx : expr * context) : expr :=
   (fix plug' e ctx :=
      match ctx with
@@ -23,21 +28,76 @@ Fixpoint plug (ectx : expr * context) : expr :=
        | app_r v ctx' =>
          e_app v (plug' e ctx')
      end)
-    (fst ectx) (snd ectx).
+    (fst ectx) (snd ectx)
+
+where "E '[' e ']'" := (plug (e, E)).
 
 Fixpoint decomp (e : expr) : (expr * context) :=
   match e with
-    | e_var x => (e, hole)
+    | e_app (e_abs x e') (e_abs x1 e1') =>
+      (e, hole)
     | e_app (e_abs x e') e2 =>
       (e2, app_r (e_abs x e') hole)
     | e_app e1 e2 =>
       (e1, app_l hole e2)
-    | e_abs x e' => (e, hole)
+    | _ => (e, hole)
   end.
 
 Lemma plug_decomp :
   forall (e : expr),
-    plug (decomp e) = e.
+      plug (decomp e) = e.
 Proof.
-  intros. induction e; try destruct e1; reflexivity.
+  intros.
+  destruct e;
+    try destruct e1; try destruct e2;
+    reflexivity.
+Qed.
+
+Reserved Notation "'[' x ':=' e' ']' e" (at level 20).
+
+Fixpoint subst (e : expr) (x : id) (e' : expr) : expr :=
+  match e with
+    | e_var x' =>
+      if beq_nat x x' then e' else e
+    | e_abs x' e1 =>
+      e_abs x' (if beq_nat x x' then e1 else ([x:=e'] e1))
+    | e_app e1 e2 =>
+      e_app ([x:=e'] e1) ([x:=e'] e2)
+  end
+
+where "'[' x ':=' e' ']' e" := (subst e x e').
+
+Reserved Notation "e '==>' e'" (at level 40).
+
+Inductive step : expr -> expr -> Prop :=
+  | E_App :
+      forall x e' v,
+        value v ->
+        (e_app (e_abs x e') v) ==> [x:=v]e'
+
+where "e '==>' e'" := (step e e').
+
+Reserved Notation "e '-->' e'" (at level 40).
+
+Inductive std_step : expr -> expr -> Prop :=
+  | StdRed :
+      forall (e : expr) (E : context) (e1 e1' : expr),
+        (e1, E) = decomp e ->
+        e1 ==> e1' ->
+        E[e1] --> E[e1']
+
+where "e '-->' e'" := (std_step e e').
+
+Example ex1 :
+  (e_app (e_abs 1 (e_abs 0 (e_var 1))) (e_abs 2 (e_var 2)))
+    --> (e_abs 0 (e_abs 2 (e_var 2))).
+Proof.
+  remember (e_app (e_abs 1 (e_abs 0 (e_var 1))) (e_abs 2 (e_var 2))) as e.
+  remember (e_abs 0 (e_abs 2 (e_var 2))) as e'.
+  remember (hole) as E.
+  assert (H1: e = E[e]) by (subst; reflexivity); rewrite H1.
+  assert (H2: e' = E[e']) by (subst; reflexivity); rewrite H2.
+  apply StdRed with (e:=e).
+  - subst. reflexivity.
+  - subst. apply E_App. apply v_abs.
 Qed.
